CertiGC/verif_resume.v
@@ -6,9 +6,15 @@ Proof.
   unfold thread_info_rep. destruct (Val.eq (ti_heap_p t_info) nullval).
   1: hnf in e; exfalso; tauto. clear n. Intros. unfold heap_struct_rep. forward. 
   unfold fun_info_rep. forward. 1: entailer!. rewrite Znth_0_cons.
+  replace_SEP 1 (fun_info_rep rsh f_info fi) by unfold fun_info_rep; entailer!.
   forward_if True; [forward; entailer!|exfalso; destruct t_info; simpl in *; tauto|].
-  Intros. remember (ti_heap_p t_info) as h. remember (ti_heap t_info) as theap.
-  pose proof (sound_gg g). simpl in H1.
+  Intros. remember (ti_heap_p t_info) as h. remember (ti_heap t_info) as th.
   forward; rewrite Znth_0_cons.
-  - entailer!.
+  - (* goal: is_pointer_or_null (space_start (heap_head (ti_heap t_info))) *)
+
+    destruct H as [? [? ?]]. rewrite <- Heqh in *. rewrite <- Heqth in *.
+    remember (glabel g) as ginfo. destruct ginfo.
+    1: exfalso; apply H1; rewrite <- H; reflexivity. simpl in H2.
+    admit.
+  - 
 Abort.
